Stating the main theorem.

concurrency/compiler/concurrent_compiler_simulation.v
@@ -9,30 +9,24 @@ Require Import VST.concurrency.compiler.HybridMachine_simulation.
 (*Clight Machine *)
 Require Import VST.concurrency.common.DryMachineSource.
 (*Asm Machine*)
-Require Import VST.concurrency.common.dry_context.
+Require Import VST.concurrency.common.x86_context.
 
 
 Section ConcurrentCopmpilerSpecification.
   (*Import the Clight Hybrid Machine*)
   Import THE_DRY_MACHINE_SOURCE.
-  Import DMS.
+  Import DMS.  
+  (*Import the Asm X86 Hybrid Machine*)
+  Import X86Context.
 
   (*Import the Asm Hybrid Machine*)
-  Import AsmContext.
   Context (Clight_g : Clight.genv).
   Context (Asm_g : Clight.genv).
-
-  (*TODO: Define this thing!!! *)
-  Context (Asm_semantics : Semantics).
-
-
-  (* Definition ClightConcurSem := @ClightMachine Clight_g. *)
-  Definition AsmHybridMachine    := @dryCoarseMach Asm_semantics.
-  Definition AsmConcurSem    := HybridMachineSig.HybridMachineSig.ConcurMachineSemantics
-                                  (HybridMachine:= AsmHybridMachine).
+  Context (Asm_program: Asm.program).
+  Context (Asm_genv_safe: Asm_core.safe_genv (the_ge Asm_program)).
 
   Definition ConcurrentCompilerCorrectness_specification: Type:=
     forall U,
-      HybridMachine_simulation (ClightConcurSem(ge:=Clight_g) U) (AsmConcurSem U).
+      HybridMachine_simulation (ClightConcurSem(ge:=Clight_g) U) (AsmConcurSem Asm_program Asm_genv_safe U).
 
 End ConcurrentCopmpilerSpecification.
