concurrency/compiler/concurrent_compiler_safety_proof.v
@@ -1,0 +1,46 @@
+
+Require Import VST.concurrency.compiler.concurrent_compiler_simulation.
+Require Import VST.concurrency.compiler.sequential_compiler_correct.
+Require Import VST.concurrency.compiler.concurrent_compiler_safety.
+Require Import VST.concurrency.compiler.concurrent_compiler_simulation_proof.
+
+
+(*Clight Machine *)
+Require Import VST.concurrency.common.DryMachineSource.
+(*Asm Machine*)
+Require Import VST.concurrency.common.x86_context.
+
+Module Concurrent_Safety (CC_correct: CompCert_correctness).
+  (*Import the Clight Hybrid Machine*)
+  Import THE_DRY_MACHINE_SOURCE.
+  Import DMS.
+  (*Import the Asm X86 Hybrid Machine*)
+  Import X86Context.
+  
+  Module ConcurCC_correct:= (Concurrent_correctness CC_correct).
+  Import ConcurCC_correct.
+
+  Parameter init_state_source:
+    forall p,
+    Clight.genv -> Memory.mem -> @semantics.semC (@DSem (Clight.globalenv p)) -> Values.val -> list Values.val -> Prop.
+  
+  Search semantics.Semantics.
+  Lemma ConcurrentCompilerSafety:
+    forall (p : Clight.program) (tp : Asm.program),
+       CC_correct.CompCert_compiler p = Some tp ->
+       forall asm_genv_safety : Asm_core.safe_genv (the_ge tp),
+         let SemSource:= (ClightSemantincsForMachines.ClightSem (Clight.globalenv p)) in
+         let SemTarget:= X86Sem tp asm_genv_safety in
+    concurrent_simulation_safety_preservation_export 
+      (SemSource:= SemSource)
+      (SourceThreadPool:= threadPool.OrdinalPool.OrdinalThreadPool(Sem:=SemSource))
+      (SourceMachineSig:= HybridMachine.DryHybridMachine.DryHybridMachineSig)
+      (SemTarget :=  SemTarget)
+      (TargetThreadPool:= threadPool.OrdinalPool.OrdinalThreadPool(Sem:=SemTarget))
+      (TargetMachineSig:= HybridMachine.DryHybridMachine.DryHybridMachineSig)
+      (init_state_source p)
+  .
+    unfold concurrent_simulation_safety_preservation; simpl; intros.
+  Admitted.
+      
+End Concurrent_Safety.
