concurrency/compiler/concurrent_compiler_simulation_proof.v
@@ -1,0 +1,14 @@
+Require Import VST.concurrency.compiler.concurrent_compiler_simulation.
+Require Import VST.concurrency.compiler.sequential_compiler_correct.
+
+
+Module Concurrent_correctness (CC_correct: CompCert_correctness).
+  
+  Lemma ConcurrentCompilerCorrectness:
+    forall (p:Clight.program) (tp:Asm.program),
+      CC_correct.CompCert_compiler p = Some tp ->
+      forall asm_genv_safety,
+        ConcurrentCompilerCorrectness_specification (Clight.globalenv p) tp asm_genv_safety.
+  Proof.
+  Admitted.
+End Concurrent_correctness.
