concurrency/compiler/sequential_compiler_correct.v
@@ -11,4 +11,5 @@ Hypothesis simpl_clight_semantic_preservation:
   CompCert_compiler p = Some tp ->
   fsim_properties_inj (Clight.semantics2 p) (Asm.semantics tp) Clight.get_mem Asm.get_mem.
 
+
 End CompCert_correctness.
